

# Mathématiques discrètes et applications

## Discrete Mathematics and Applications

Problem Session 3

Peterson Yuhala

Instituts d'informatique et de mathématiques  
Université de Neuchâtel

Automne 2025 / Fall 2025



# Contact information

Peterson Yuhala

Office B119

[peterson.yuhala@unine.ch](mailto:peterson.yuhala@unine.ch)

## Ex-1: Quantified statements.

$$(a) \exists x(C(x) \wedge D(x) \wedge F(x))$$

$$(b) \forall x(C(x) \vee D(x) \vee F(x))$$

$$(c) \exists x(C(x) \wedge F(x) \wedge \neg D(x))$$

$$(d) \neg \exists x(C(x) \wedge D(x) \wedge F(x)) \equiv \forall x(\neg C(x) \vee \neg D(x) \vee \neg F(x))$$

$$(e) \exists xC(x) \wedge \exists yD(y) \wedge \exists zF(z) \equiv \exists x\exists y\exists z(C(x) \wedge D(y) \wedge F(z))$$

We can also write the proposition as:

$\exists xC(x) \wedge \exists xD(x) \wedge \exists xF(x)$ . Note that  $x$  can refer to a different person in each term.

## Ex-2: Quantified statements.

(a)  $\forall x F(x, \text{Nancie})$

(b)  $\forall y F(\text{Peter}, y)$

(c)  $\forall x \exists y F(x, y)$

(d)  $\neg \exists x \forall y F(x, y) \equiv \forall x \exists y \neg F(x, y)$

(e)  $\forall y \exists x F(x, y)$

(f)

$$\begin{aligned}\neg \exists x (F(x, \text{Ouny}) \wedge F(x, \text{Leyla})) &\equiv \forall x \neg (F(x, \text{Ouny}) \wedge F(x, \text{Leyla})) \\ &\equiv \forall x (\neg F(x, \text{Ouny}) \vee \neg F(x, \text{Leyla}))\end{aligned}$$

## Ex-2: Quantified statements.

$$(g) \exists y_1 \exists y_2 (y_1 \neq y_2 \wedge F(Essil, y_1) \wedge F(Essil, y_2) \wedge \forall y (F(Essil, y) \rightarrow (y = y_1 \vee y = y_2)))$$

$$(h) \neg \exists y F(Ehlana, y) \equiv \forall y \neg F(Ehlana, y)$$

$$(i) \exists! y \forall x F(x, y) \equiv \exists y (\forall x F(x, y) \wedge \forall z (\forall w F(w, z) \rightarrow y = z))$$

$$(j) \forall x \neg F(x, x)$$

$$(k) \exists x \exists y (x \neq y \wedge F(x, y) \wedge \forall z (F(x, z) \rightarrow z = y))$$

## Ex-3: Definition of a limit

· We have:  $\lim_{x \rightarrow a} f(x) = L \iff$

$$\forall \varepsilon > 0 \exists \delta > 0 \forall x |x - a| < \delta \rightarrow |f(x) - L| < \varepsilon$$

· If we name the proposition on the right  $P$ , then  $\lim_{x \rightarrow a} f(x) \neq L$  can be interpreted as  $\neg P$ .

· Thus we have  $\neg P$  as:

$$\begin{aligned}\neg P &\equiv \neg(\forall \varepsilon > 0 \exists \delta > 0 \forall x |x - a| < \delta \rightarrow |f(x) - L| < \varepsilon) \\ &\equiv \exists \varepsilon > 0 \forall \delta > 0 \exists x (|x - a| < \delta \wedge |f(x) - L| \geq \varepsilon)\end{aligned}$$

· Note that the restricted domains (e.g.,  $\varepsilon > 0$  or  $\delta > 0$ ) on which the quantifiers apply are not changed when the negation is done. However, we negate the conditional statement being quantified.

## Ex-4: Rules of Inference

Consider the following statements:

$p$  : It's sunny this afternoon.

$q$  : It's colder than yesterday.

$r$  : We will go swimming.

$s$  : We will take a canoe trip.

$t$  : We will be home by sunset.

### Premises:

1.  $\neg p \wedge q$

2.  $r \rightarrow p$

3.  $\neg r \rightarrow s$

4.  $s \rightarrow t$

**Conclusion:**  $t$

## Ex-4: Rules of Inference

We construct our argument with the premises and rules of inference to arrive at the conclusion.

Step	Reason
$\neg r \rightarrow s$	Premise 3
$s \rightarrow t$	Premise 4
$\neg r \rightarrow t$	Transitivity/Hypothetical syllogism
$\neg p \wedge q$	Premise 1
$\neg p$	Specialization/Simplification
$r \rightarrow p$	Premise 2
$\neg r$	Modus Tollens
$t$	Modus Ponens (see $\neg r \rightarrow t$ above)



## Ex-5: Mathematical Induction

Let  $P(n)$  be the statement:  $\forall n \in \mathbb{N}$ ,  $n(n+1)(n+2)$  is divisible by 6.

**Basis Step:**  $n = 0$

$P(0)$ :  $0(0+1)(0+2) = 0$ , which is divisible by 6. So  $P(0)$  is true.

**Inductive Step:** We assume  $P(k)$  is true for an arbitrary  $k \geq 0$ , which is our inductive hypothesis (I.H.):

$P(k)$ :  $k(k+1)(k+2)$  is divisible by 6.

Assuming the I.H., we show that  $P(k+1)$  is true.

· **NB:** The truth of  $P(k+1)$  must follow from the I.H., i.e., from the truth of  $P(k)$ . You do not show that  $P(k+1)$  is true on its own.

## Ex-5: Mathematical Induction

$$\begin{aligned}P(k+1) : (k+1)(k+2)(k+3) &= k(k+1)(k+2) + 3(k+1)(k+2) \\&\stackrel{\text{I.H}}{=} 6M + 3(k+1)(k+2), \quad M \in \mathbb{Z} \\&\stackrel{(*)}{=} 6M + 3 \cdot 2 \cdot N, \quad N \in \mathbb{Z} \\&= 6M + 6N \\&= 6(M+N)\end{aligned}$$

For the equality  $(*)$ , we have used that  $(k+1)(k+2)$  is even, so  $(k+1)(k+2) = 2N$  for some  $N \in \mathbb{Z}$ .

$6(M+N)$  is divisible by 6. Therefore  $P(k) \rightarrow P(k+1)$ , and by the principle of mathematical induction,  $\forall n \in \mathbb{N}$ ,  $P(n)$  holds.

## Ex-6: Proof by Contradiction

- To prove a proposition  $P$  by contradiction, we show that  $\neg P \rightarrow \mathbf{F}$ . In other words, by assuming  $P$  is false, we arrive at a contradiction.
- This indirectly proves  $P$  because  $P \equiv (\neg P \rightarrow \mathbf{F})$ .
- This proof method also applies if  $P$  is a conditional statements/proposition of the form  $A \rightarrow B$ .

· So to prove by contradiction that:  $\forall a \in \mathbb{Z}, a^2 \text{ even} \rightarrow a \text{ even}$ , we show that the hypothesis  $\neg(\forall a \in \mathbb{Z}, a^2 \text{ even} \rightarrow a \text{ even})$  leads to a contradiction.

·  $\neg(\forall a \in \mathbb{Z}, a^2 \text{ even} \rightarrow a \text{ even}) \equiv \exists a \in \mathbb{Z} \mid (a^2 \text{ even} \wedge a \text{ odd})$ .

$$a \text{ odd} \implies \exists c \in \mathbb{Z} \text{ such that } a = 2c + 1$$

$$\implies a^2 = 4c^2 + 4c + 1 = 2(2c^2 + 2c) + 1 \text{ is odd}$$

· We have both  $a^2$  even and  $a^2$  odd, hence a contradiction. So  $P$  is true.

## Ex-7: Proof by Contraposition.

· To prove that  $P \rightarrow Q$  by contraposition, we show that  $\neg Q \rightarrow \neg P$ . This proof method is valid because a conditional statement is logically equivalent to its contrapositive.

Consider (for some arbitrary, but fixed  $a$ ,  $b$ , and  $n$ ) the following statements:  $p: n = ab$ ,  $q: a \leq \sqrt{n}$ , and  $r: b \leq \sqrt{n}$ .

We want to prove that:  $p \rightarrow (q \vee r)$ .

By contraposition, it suffices to show that  $\neg(q \vee r) \rightarrow \neg p$ .

$$\begin{aligned}\neg(q \vee r) &\equiv \neg q \wedge \neg r \\ &= (a > \sqrt{n}) \wedge (b > \sqrt{n}) \\ &\implies ab > \sqrt{n}\sqrt{n} = n \\ &\implies ab \neq n\end{aligned}$$

i.e  $\neg(q \vee r) \rightarrow \neg p$ .



## Ex-8: Mathematical Induction

Let  $P(n)$  be the statement:

$$\forall n \geq 1, \forall (p_1, \dots, p_n) \in \{0, 1\}^n : \neg(p_1 \wedge \dots \wedge p_n) = \neg p_1 \vee \dots \vee \neg p_n$$

**Basis Step:** For  $n = 1$ ,  $\neg p_1 = \neg p_1$ , so  $P(1)$  is true (there is nothing to do).

For  $n = 2$ ,  $\neg(p_1 \wedge p_2) = \neg p_1 \vee \neg p_2$  (shown using truth tables). So also  $P(2)$  is true.

**Inductive Step:** We assume  $P(k)$  is true for an arbitrary  $k \geq 2$  (Inductive Hypothesis):

$$P(k) : \forall (p_1, \dots, p_k) \in \{0, 1\}^k : \neg(p_1 \wedge \dots \wedge p_k) = \neg p_1 \vee \dots \vee \neg p_k$$

and show that if  $P(k)$  is true, then  $P(k+1)$  is true.

$P(k+1)$  is the following statement:

$$\begin{aligned} & \forall (p_1, \dots, p_{k+1}) \in \{0, 1\}^{k+1} : \\ & \neg(p_1 \wedge \dots \wedge p_k \wedge p_{k+1}) = \neg p_1 \vee \dots \vee \neg p_k \vee \neg p_{k+1} \end{aligned}$$

## Ex-8: Mathematical Induction

$$\begin{aligned}\neg(p_1 \wedge \dots \wedge p_k \wedge p_{k+1}) &= \neg((p_1 \wedge p_2 \wedge \dots \wedge p_k) \wedge p_{k+1}) \\ &= \neg(p_1 \wedge \dots \wedge p_k) \vee \neg p_{k+1} && \text{case } n = 2 \\ &\stackrel{\text{I.H}}{=} (\neg p_1 \vee \dots \vee \neg p_k) \vee \neg p_{k+1} \\ &= \neg p_1 \vee \dots \vee \neg p_k \vee \neg p_{k+1}\end{aligned}$$

Therefore  $P(k) \rightarrow P(k+1)$  and by the principle of mathematical induction,  $\forall n \in \mathbb{N}$ ,  $P(n)$  holds.

TODO at home: Similar proof for the second law.

## Ex-9: Proving conjectures by mathematical induction.

By computing the sum for small values of  $n$ , we can conjecture that the following statement  $P(n)$  holds for all  $n$ :

$$P(n) : \sum_{i=1}^n \frac{1}{2^i} = \frac{2^n - 1}{2^n}$$

Let us prove our conjecture by mathematical induction.

**Basis Step:**  $n = 1$

$P(1)$ :  $\frac{1}{2^1} = \frac{2^1 - 1}{2^1} = \frac{1}{2}$ . So  $P(1)$  is true.

**Inductive Step:** We assume  $P(k)$  is true for an arbitrary  $k \geq 1$   
(I.H.)

$$P(k) : \sum_{i=1}^k \frac{1}{2^i} = \frac{2^k - 1}{2^k}$$

Assuming the I.H., we show that  $P(k+1)$  is true.

## Ex-9: Proving conjectures by mathematical induction.

$$\begin{aligned}P(k+1) : \sum_{i=1}^{k+1} \frac{1}{2^i} &= \sum_{i=1}^k \frac{1}{2^i} + \frac{1}{2^{k+1}} \\&\stackrel{\text{I.H.}}{=} \frac{2^k - 1}{2^k} + \frac{1}{2^{k+1}} \\&= \frac{2(2^k - 1) + 1}{2^{k+1}} \\&= \frac{2 \cdot 2^k - 2 + 1}{2} \\&= \frac{2^{k+1} - 1}{2^{k+1}}\end{aligned}$$

Therefore  $P(k) \rightarrow P(k+1)$ , and by the principle of mathematical induction,  $\forall n \in \mathbb{N}$ ,  $P(n)$  holds.



# End

For more exercises and notes, see Rosen 7th Edition  
Chap. 1.4-1.8 and Chap. 5.1.